change CRC-32 to CRC-32C, add a c++ implementation for CRC-32C

disk-betree/Crc32.cpp
@@ -1,0 +1,49 @@
+// Needs to be compiled with -msse4.2
+
+#include <iostream>
+#include <cstring>
+#include <smmintrin.h>
+
+using namespace std;
+
+uint32_t crc32c(const uint8_t *bytes, size_t len)
+{
+  uint32_t acc = 0xffffffff;
+
+  while (((uintptr_t)bytes) & 0x7 && len > 0) {
+    acc = _mm_crc32_u8(acc, *bytes);
+    bytes++;
+    len--;
+  }
+
+  while (len >= 8) {
+    acc = _mm_crc32_u64(acc, *((const uint64_t *)bytes));
+    len -= 8;
+    bytes += 8;
+  }
+
+  if (len >= 4) {
+    acc = _mm_crc32_u32(acc, *((const uint32_t *)bytes));
+    len -= 4;
+    bytes += 4;
+  }
+
+  if (len >= 2) {
+    acc = _mm_crc32_u16(acc, *((const uint16_t *)bytes));
+    len -= 2;
+    bytes += 2;
+  }
+
+  if (len >= 1) {
+    acc = _mm_crc32_u8(acc, *bytes);
+    len -= 1;
+    bytes += 1;
+  }
+
+  return ~acc;
+}
+
+int main() {
+  const char* ch = "The quick brown fox jumps over the lazy dog";
+	cout << crc32c((const uint8_t*)ch, strlen(ch)) << endl;
+}
