lib/Base/Crypto.s.dfy
@@ -6,12 +6,15 @@ module {:extern} Crypto {
   function method {:axiom} Sha256(t: seq<byte>) : (hash : seq<byte>)
   ensures |hash| == 32
 
-  function method {:axiom} Crc32(t: seq<byte>) : (hash : seq<byte>)
+  // NOTE: The CRC-32C checksum is a 4-byte checksum; the value returned
+  // by this function is padded up to 32 bytes.
+  // TODO: don't do this, just return 4 bytes instead.
+  function method {:axiom} Crc32C(t: seq<byte>) : (hash : seq<byte>)
   ensures |hash| == 32
 
-  method {:axiom} Crc32Array(t: array<byte>, start: uint64, len: uint64)
+  method {:axiom} Crc32CArray(t: array<byte>, start: uint64, len: uint64)
   returns (hash : seq<byte>)
   requires 0 <= start
   requires start as int + len as int <= t.Length
-  ensures hash == Crc32(t[start .. start as int + len as int])
+  ensures hash == Crc32C(t[start .. start as int + len as int])
 }
